src/JSON/JSON.Serializer.dfy
@@ -37,31 +37,31 @@ module {:options "-functionSyntax:4"} JSON.Serializer {
     ensures wr.Bytes() == writer.Bytes() + Spec.Value(v)
   {
     match v
-      case Null(n) =>
-        writer.Append(n)
-      case Bool(b) =>
-        writer.Append(b)
-      case String(str) =>
-        writer.Append(str)
-      case Number(minus, num, frac, exp) =>
-        Number(v, writer)
-      case Object(obj) =>
-        Object(v, obj, writer)
-      case Array(arr) =>
-        Array(v, arr, writer)
+      case Null(n) => writer.Append(n)
+      case Bool(b) => writer.Append(b)
+      case String(str) => String(str, writer)
+      case Number(num) => Number(num, writer)
+      case Object(obj) => Object(obj, writer)
+      case Array(arr) => Array(arr, writer)
   }
 
-  function {:opaque} Number(v: Value, writer: Writer) : (wr: Writer)
-    requires v.Number?
-    decreases v, 0
-    ensures wr.Bytes() == writer.Bytes() + Spec.Value(v)
+  function {:opaque} String(str: jstring, writer: Writer) : (wr: Writer)
+    decreases str, 0
+    ensures wr.Bytes() == writer.Bytes() + Spec.String(str)
   {
-    var writer := writer.Append(v.minus).Append(v.num);
-    var writer := if v.frac.NonEmpty? then
-        writer.Append(v.frac.t.period).Append(v.frac.t.num)
+    writer.Append(str)
+  }
+
+  function {:opaque} Number(num: jnumber, writer: Writer) : (wr: Writer)
+    decreases num, 0
+    ensures wr.Bytes() == writer.Bytes() + Spec.Number(num)
+  {
+    var writer := writer.Append(num.minus).Append(num.num);
+    var writer := if num.frac.NonEmpty? then
+        writer.Append(num.frac.t.period).Append(num.frac.t.num)
       else writer;
-    var writer := if v.exp.NonEmpty? then
-        writer.Append(v.exp.t.e).Append(v.exp.t.sign).Append(v.exp.t.num)
+    var writer := if num.exp.NonEmpty? then
+        writer.Append(num.exp.t.e).Append(num.exp.t.sign).Append(num.exp.t.num)
       else writer;
     writer
   }
@@ -77,145 +77,163 @@ module {:options "-functionSyntax:4"} JSON.Serializer {
 
   // FIXME refactor below to merge
 
-  function {:opaque} Object(v: Value, obj: jobject, writer: Writer) : (wr: Writer)
-    requires v.Object? && obj == v.obj
-    decreases v, 3
-    ensures wr.Bytes() == writer.Bytes() + Spec.Value(v)
+  function {:opaque} Object(obj: jobject, writer: Writer) : (wr: Writer)
+    decreases obj, 3
+    ensures wr.Bytes() == writer.Bytes() + Spec.Object(obj)
   {
     var writer := StructuralView(obj.l, writer);
-    var writer := Members(v, obj, writer);
+    var writer := Members(obj, writer);
     var writer := StructuralView(obj.r, writer);
 
     // We call ``ConcatBytes`` with ``Spec.Member``, whereas the spec calls it
     // with ``(d: jmember) requires d in obj.data => Spec.Member(d)``.  That's
     // why we need an explicit cast, which is performed by the lemma below.
     SpecProperties.Bracketed_Morphism(obj);
-    assert Spec.Value(v) == Spec.Bracketed(obj, Spec.Member);
+    assert Spec.Object(obj) == Spec.Bracketed(obj, Spec.Member);
     writer
   }
 
-  function {:opaque} Array(v: Value, arr: jarray, writer: Writer) : (wr: Writer)
-    requires v.Array? && arr == v.arr
-    decreases v, 3
-    ensures wr.Bytes() == writer.Bytes() + Spec.Value(v)
+  function {:opaque} Array(arr: jarray, writer: Writer) : (wr: Writer)
+    decreases arr, 3
+    ensures wr.Bytes() == writer.Bytes() + Spec.Array(arr)
   {
     var writer := StructuralView(arr.l, writer);
-    var writer := Items(v, arr, writer);
+    var writer := Items(arr, writer);
     var writer := StructuralView(arr.r, writer);
 
     // We call ``ConcatBytes`` with ``Spec.Item``, whereas the spec calls it
     // with ``(d: jitem) requires d in arr.data => Spec.Item(d)``.  That's
     // why we need an explicit cast, which is performed by the lemma below.
     SpecProperties.Bracketed_Morphism(arr); // DISCUSS
-    assert Spec.Value(v) == Spec.Bracketed(arr, Spec.Item);
+    assert Spec.Array(arr) == Spec.Bracketed(arr, Spec.Item);
     writer
   }
 
-  function {:opaque} Members(ghost v: Value, obj: jobject, writer: Writer) : (wr: Writer)
-    requires obj < v
-    decreases v, 2
+  function {:opaque} Members(obj: jobject, writer: Writer) : (wr: Writer)
+    decreases obj, 2
     ensures wr.Bytes() == writer.Bytes() + Spec.ConcatBytes(obj.data, Spec.Member)
   {
-    MembersSpec(v, obj.data, writer)
+    MembersSpec(obj, obj.data, writer)
   } by method {
-    wr := MembersImpl(v, obj, writer);
-    Assume(false); // FIXME
+    wr := MembersImpl(obj, writer);
+    Assume(false); // BUG(https://github.com/dafny-lang/dafny/issues/2180)
   }
 
-  function {:opaque} Items(ghost v: Value, arr: jarray, writer: Writer) : (wr: Writer)
-    requires arr < v
-    decreases v, 2
+  function {:opaque} Items(arr: jarray, writer: Writer) : (wr: Writer)
+    decreases arr, 2
     ensures wr.Bytes() == writer.Bytes() + Spec.ConcatBytes(arr.data, Spec.Item)
   {
-    ItemsSpec(v, arr.data, writer)
+    ItemsSpec(arr, arr.data, writer)
   } by method {
-    wr := ItemsImpl(v, arr, writer);
-    Assume(false); // FIXME
+    wr := ItemsImpl(arr, writer);
+    Assume(false); // BUG(https://github.com/dafny-lang/dafny/issues/2180)
   }
 
-  ghost function MembersSpec(v: Value, members: seq<jmember>, writer: Writer) : (wr: Writer)
-    requires forall j | 0 <= j < |members| :: members[j] < v
-    decreases v, 1, members
+  ghost function MembersSpec(obj: jobject, members: seq<jmember>, writer: Writer) : (wr: Writer)
+    requires forall j | 0 <= j < |members| :: members[j] < obj
+    decreases obj, 1, members
     ensures wr.Bytes() == writer.Bytes() + Spec.ConcatBytes(members, Spec.Member)
   { // TR elimination doesn't work for mutually recursive methods, so this
     // function is only used as a spec for Members.
     if members == [] then writer
     else
-      var writer := MembersSpec(v, members[..|members|-1], writer);
+      var writer := MembersSpec(obj, members[..|members|-1], writer);
       assert members == members[..|members|-1] + [members[|members|-1]];
       SpecProperties.ConcatBytes_Linear(members[..|members|-1], [members[|members|-1]], Spec.Member);
-      Member(v, members[|members|-1], writer)
+      Member(obj, members[|members|-1], writer)
   } // No by method block here, because the loop invariant in the method version
     // needs to call MembersSpec and the termination checker gets confused by
     // that.  Instead, see Members above. // DISCUSS
 
-  ghost function ItemsSpec(v: Value, items: seq<jitem>, writer: Writer) : (wr: Writer)
-    requires forall j | 0 <= j < |items| :: items[j] < v
+  // DISCUSS: Is there a way to avoid passing the ghost `v` around while
+  // maintaining the termination argument?  Maybe the lambda for elements will be enough?
+
+  ghost function SequenceSpec<T>(v: Value, items: seq<T>,
+                                 spec: T -> bytes, impl: (ghost Value, T, Writer) --> Writer,
+                                 writer: Writer)
+    : (wr: Writer)
+    requires forall item, wr | item in items :: impl.requires(v, item, wr)
+    requires forall item, wr | item in items :: impl(v, item, wr).Bytes() == wr.Bytes() + spec(item)
     decreases v, 1, items
+    ensures wr.Bytes() == writer.Bytes() + Spec.ConcatBytes(items, spec)
+  { // TR elimination doesn't work for mutually recursive methods, so this
+    // function is only used as a spec for Items.
+    if items == [] then writer
+    else
+      var writer := SequenceSpec(v, items[..|items|-1], spec, impl, writer);
+      assert items == items[..|items|-1] + [items[|items|-1]];
+      SpecProperties.ConcatBytes_Linear(items[..|items|-1], [items[|items|-1]], spec);
+      impl(v, items[|items|-1], writer)
+  } // No by method block here, because the loop invariant in the method version
+    // needs to call `SequenceSpec` and the termination checker gets confused by
+    // that.  Instead, see `Sequence`Items above. // DISCUSS
+
+
+  ghost function ItemsSpec(arr: jarray, items: seq<jitem>, writer: Writer) : (wr: Writer)
+    requires forall j | 0 <= j < |items| :: items[j] < arr
+    decreases arr, 1, items
     ensures wr.Bytes() == writer.Bytes() + Spec.ConcatBytes(items, Spec.Item)
   { // TR elimination doesn't work for mutually recursive methods, so this
     // function is only used as a spec for Items.
     if items == [] then writer
     else
-      var writer := ItemsSpec(v, items[..|items|-1], writer);
+      var writer := ItemsSpec(arr, items[..|items|-1], writer);
       assert items == items[..|items|-1] + [items[|items|-1]];
       SpecProperties.ConcatBytes_Linear(items[..|items|-1], [items[|items|-1]], Spec.Item);
-      Item(v, items[|items|-1], writer)
+      Item(arr, items[|items|-1], writer)
   } // No by method block here, because the loop invariant in the method version
     // needs to call ItemsSpec and the termination checker gets confused by
     // that.  Instead, see Items above. // DISCUSS
 
-  method MembersImpl(ghost v: Value, obj: jobject, writer: Writer) returns (wr: Writer)
-    requires obj < v
-    decreases v, 1
-    ensures wr == MembersSpec(v, obj.data, writer);
+  method MembersImpl(obj: jobject, writer: Writer) returns (wr: Writer)
+    decreases obj, 1
+    ensures wr == MembersSpec(obj, obj.data, writer);
   {
     wr := writer;
     var members := obj.data;
-    assert wr == MembersSpec(v, members[..0], writer);
+    assert wr == MembersSpec(obj, members[..0], writer);
     for i := 0 to |members| // FIXME uint32
-      invariant wr == MembersSpec(v, members[..i], writer)
+      invariant wr == MembersSpec(obj, members[..i], writer)
     {
       assert members[..i+1][..i] == members[..i];
-      wr := Member(v, members[i], wr);
+      wr := Member(obj, members[i], wr);
     }
     assert members[..|members|] == members;
   }
 
-  method ItemsImpl(ghost v: Value, arr: jarray, writer: Writer) returns (wr: Writer)
-    requires arr < v
-    decreases v, 1
-    ensures wr == ItemsSpec(v, arr.data, writer);
+  method ItemsImpl(arr: jarray, writer: Writer) returns (wr: Writer)
+    decreases arr, 1
+    ensures wr == ItemsSpec(arr, arr.data, writer);
   {
     wr := writer;
     var items := arr.data;
-    assert wr == ItemsSpec(v, items[..0], writer);
+    assert wr == ItemsSpec(arr, items[..0], writer);
     for i := 0 to |items| // FIXME uint32
-      invariant wr == ItemsSpec(v, items[..i], writer)
+      invariant wr == ItemsSpec(arr, items[..i], writer)
     {
       assert items[..i+1][..i] == items[..i];
-      wr := Item(v, items[i], wr);
+      wr := Item(arr, items[i], wr);
     }
     assert items[..|items|] == items;
   }
 
-  function {:opaque} Member(ghost v: Value, m: jmember, writer: Writer) : (wr: Writer)
-    requires m < v
-    decreases v, 0
+  function {:opaque} Member(ghost obj: jobject, m: jmember, writer: Writer) : (wr: Writer)
+    requires m < obj
+    decreases obj, 0
     ensures wr.Bytes() == writer.Bytes() + Spec.Member(m)
   {
-    var writer := if m.prefix.Empty? then writer else StructuralView(m.prefix.t, writer);
     var writer := writer.Append(m.t.k);
     var writer := StructuralView(m.t.colon, writer);
-    Value(m.t.v, writer)
+    var writer := Value(m.t.v, writer);
+    if m.suffix.Empty? then writer else StructuralView(m.suffix.t, writer)
   }
 
-  function {:opaque} Item(ghost v: Value, m: jitem, writer: Writer) : (wr: Writer)
-    requires m < v
-    decreases v, 0
+  function {:opaque} Item(ghost arr: jarray, m: jitem, writer: Writer) : (wr: Writer)
+    requires m < arr
+    decreases arr, 0
     ensures wr.Bytes() == writer.Bytes() + Spec.Item(m)
   {
-    var wr := if m.prefix.Empty? then writer else StructuralView(m.prefix.t, writer);
-    Value(m.t, wr)
+    var writer := Value(m.t, writer);
+    if m.suffix.Empty? then writer else StructuralView(m.suffix.t, writer)
   }
 }
